sketch: defin tactic mode

omin/tactic.lean
@@ -56,7 +56,7 @@ meta def defin_start : tactic unit :=
 /-- Return the variable representing the definable context. -/
 meta def guess_ctx_var : tactic expr :=
 do `(o_minimal.definable_psh.definable (λ (_ : ↥%%var), _)) ← target,
---   trace var,
+   -- trace var,
    return var
 
 /-- Return a list of "definable" variables along with their processed types. -/
@@ -67,13 +67,49 @@ do l ← local_context,
      (do `(o_minimal.sect %%ctx_var %%ty) ← infer_type var,
          return $ some (var, ty)) <|> return none),
    let l' := l.filter_map id,
-   trace l',
+   -- trace l',
    return l'
 
 meta def guess_defin_vars' : tactic (list (expr × expr)) :=
 guess_ctx_var >>= guess_defin_vars
 
+/-- Goal should look like
+  ⊢ definable_psh.definable (λ γ, λ x, e)
+We want to "intro" `x` as a definable variable, and leave
+  ⊢ definable_psh.definable (λ γ, e)
+as the new goal.
+
+Strategy:
+By `definable_fun'` it's enough to check the new goal
+for an arbitrary context extension π : Γ' → Γ and section x : Γ' ⊢ α.
+However, we also have to move any existing definable variables from Γ to Γ'.
+So, we proceed as follows:
+* Identify the variables `γ` (`i_var`) and `Γ` (`ctx_var`) in the goal
+  `definable_psh.definable (λ (γ : Γ), body)`.
+  Here `body` is expected to be a function whose argument `x`
+  we want to intro.
+* Use `definable_fun'` but then intro only `Γ'` and `π`.
+* For each existing definable variable `p`, we add a let binding
+  `p' := p.precomp π`.
+* Now intro the new variable `x` (`new_var`) as well, and build a new function
+  (λ (γ' : Γ'), body' (x.to_fun γ')), by making the following replacements:
+  - each old `p` becomes `p'`;
+  - `i` becomes `i'`;
+  - `Γ` becomes `Γ'`.
+  The claim is that the new expression is well-typed and definitionally equal
+  (in the context of the let-bound variables `p'`, ...) to the current goal.
+  Moreover, it only mentions the new `Γ'` and `p'`.
+* Now we cover our tracks:
+  - clear the bodies of the let bindings `p'`, so that we can:
+  - clear the old definable variables, `π`, and the old `Γ`.
+
+The tactic reuses the same user-visible names for the new `Γ` and `γ`.
+This is nice for interactive use, but not so nice for debugging the tactic.
+In the latter case, add `name.append_after _ 1` when generating names.
+-/
 meta def defin_intro (var : parse ident_) : tactic unit :=
+let trace : Π {α : Type} [has_to_tactic_format α] (a : α), tactic unit :=
+  λ _ _ _, tactic.skip in       -- comment this for debugging
 do `(o_minimal.definable_psh.definable %%f) ← target,
    ([i_var], body) ← open_n_lambdas f 1,
    ctx_var ← guess_ctx_var,
@@ -91,10 +127,11 @@ do `(o_minimal.definable_psh.definable %%f) ← target,
      new_body ← to_expr ``((%%dvar).precomp %%proj_var),
      new_dvar ← tactic.pose dvar.local_pp_name none new_body,
      return (sigma.mk dvar new_dvar)),
-   -- * replace variables `p` → `p'` in `body`, and also the i var
    new_i_type ← to_expr ``(↥%%new_ctx_var),
    new_i_var ← mk_local' i_var.local_pp_name f.binding_info new_i_type,
-   let var_map := (defin_var_list.to_alist.insert i_var new_i_var).insert ctx_var new_ctx_var,
+   -- * replace variables `p` → `p'` in `body`, and also the γ and Γ vars
+   let var_map :=
+     (defin_var_list.to_alist.insert i_var new_i_var).insert ctx_var new_ctx_var,
    let body' := body.replace (λ e _, do
      -- for "efficiency", first check whether we have a variable at all
      guard (e.is_local_constant),
@@ -118,7 +155,137 @@ do `(o_minimal.definable_psh.definable %%f) ← target,
    tactic.clear ctx_var,
    return ()
 
+/-- Goal should look like
+ ⊢ definable_psh.definable (λ γ, f x)
+and we want to produce
+ ⊢ definable_psh.definable (λ γ, f)
+ ⊢ definable_psh.definable (λ γ, x)
+This is just `apply definable.app_ctx'`,
+but Lean needs help with the unification problem.
+-/
+meta def defin_app : tactic unit :=
+do `(o_minimal.definable_psh.definable %%e) ← target,
+   ([i_var], body) ← open_n_lambdas e 1,
+   (expr.app f x) ← pure body,
+   f' ← tactic.lambdas [i_var] f,
+   x' ← tactic.lambdas [i_var] x,
+   `[apply o_minimal.definable.app_ctx' %%f' %%x'],
+   return ()
+
+/-- Goal should look like
+ ⊢ definable_psh.definable (λ γ, p.to_fun γ)
+where p : Γ ⊢ α. Just apply `sect.definable`.
+-/
+meta def defin_var : tactic unit :=
+`[apply o_minimal.sect.definable]
+
 end tactic.interactive
+
+-- Now dress it up
+
+meta def defin := tactic
+
+meta instance : monad defin :=
+show monad tactic, by apply_instance
+
+meta instance : interactive.executor defin :=
+{ config_type := unit,
+  inhabited := by apply_instance,
+  execute_with := λ _ tac, tactic.interactive.defin_start >> tac }
+
+namespace defin
+
+meta def execute (tac : defin unit) : tactic unit :=
+tactic.interactive.defin_start >> tac
+
+meta def step := @tactic.step   -- what does this even do
+meta def istep := @tactic.istep -- ditto
+meta def solve1 : defin unit → defin unit := tactic.solve1
+
+open tactic
+
+-- Tactic state display borrows liberally from
+-- https://github.com/unitb/temporal-logic
+-- file temporal_logic.tactic
+
+/-- Replace any occurrences of `p.to_fun γ` with simply `p`.
+This is rather crude, but these aren't expected to appear
+outside the execution of a defin tactic. (More sophisticated
+would be to process only those variables which are sections
+over the context variable that appears in the goal.)
+The resulting expression is intended to be used for display purposes. -/
+meta def shorten (E : expr) : expr :=
+E.replace $ λ e _, match e with
+  | `(o_minimal.sect.to_fun %%p _) := some p
+  | _ := none
+end
+
+meta structure hyp_data : Type :=
+(crisp : bool)
+(var : expr)
+(ty : expr)
+(val : option expr)
+
+/-- Return information about a local hypothesis `l`. -/
+meta def get_hyp_data (l : expr) : defin hyp_data :=
+do ty ← infer_type l,
+   val ← try_core (shorten <$> local_def_value l),
+   match ty with
+   | `(o_minimal.sect %%Γ %%ty') := return ⟨ff, l, shorten ty', val⟩
+   | _ := return ⟨tt, l, shorten ty, val⟩
+   end
+
+meta def decl_to_fmt (s : tactic_state) (crisp : bool) (vs : list expr)
+  (ty : expr) (val : option expr) : format :=
+let vs' := format.join $ (vs.map s.format_expr).intersperse " ",
+    t := s.format_expr ty,
+    sep := if crisp then "::" else ":" in
+match val with
+| (some val) := format! "{vs'} {sep} {t} := {s.format_expr val}"
+| none := format! "{vs'} {sep} {t}"
+end
+
+meta def goal_to_fmt (g : expr) : defin (thunk format) :=
+do set_goals [g],
+   s ← read,
+   `(o_minimal.definable_psh.definable (λ (_ : ↥%%Γ), %%body)) ← target
+     | pure (λ _, to_fmt s),
+   lc ← local_context,
+   ctx_var ← tactic.interactive.guess_ctx_var,
+   dat ← (lc.filter (λ l, l ≠ ctx_var)).mmap get_hyp_data,
+   return $ λ _, format.intercalate format.line
+     [format.intercalate ("," ++ format.line) $ dat.map $ λ d,
+        decl_to_fmt s d.crisp [d.var] d.ty d.val,
+      format! "⊢ {s.format_expr (shorten body)} def"]
+
+meta def save_info (p : pos) : defin unit :=
+do gs ← get_goals,
+   fmt ← gs.mmap goal_to_fmt,
+   set_goals gs,
+   tactic.save_info_thunk p (λ _,
+     let header := if fmt.length > 1 then format! "{fmt.length} goals\n" else "",
+         eval : thunk format → format := λ f, f () in
+     if fmt.empty
+       then "no goals"
+       else format.join ((fmt.map eval).intersperse (format.line ++ format.line)))
+
+namespace interactive
+
+meta def swap := tactic.interactive.swap
+meta def exact := tactic.interactive.exact
+meta def solve1 : defin unit → defin unit := tactic.interactive.solve1
+
+meta def intro := tactic.interactive.defin_intro
+meta def app := tactic.interactive.defin_app
+meta def var := tactic.interactive.defin_var
+
+meta def trace_state : defin unit :=
+do s ← read,
+   trace s.to_format
+
+end interactive
+
+end defin
 
 namespace o_minimal
 
@@ -126,61 +293,37 @@ variables {R : Type*} {S : struc R}
 
 local infixr ` ⊢ `:10 := sect
 
---set_option pp.all true
 example : definable S (λ p q, (q ∧ p) ∧ q) :=
 begin
   defin_start,
-
-  --guess_ctx_var,
-  --guess_defin_vars',
-
-  -- "intro p",
-/-
-  rw definable_fun', intros Γ' π p,
-  -- now we need to pull back any variables mentioning Γ
-  -- to use Γ' -- there aren't any yet ✓
-  -- since that's done, we can dispose of the old context
-  clear π Γ,
--/
   defin_intro p,
-
-  -- "intro q",
-/-
-  rw definable_fun', intros Γ_1_1 π, -- don't intro q just yet
-  -- this time we need to deal with p
-  let p_1 := p.precomp π,
-  intro q,
-  change (definable_psh.definable (λ γ_1, (q.to_fun γ_1 ∧ p_1.to_fun γ_1) ∧ q.to_fun γ_1)),
-  -- dispose of old context again
-  clear_value p_1,
-  clear p π Γ_1,
-  rename Γ' → Γ,
--/
   defin_intro q,
-
-  -- we're done with intros!
-
-  -- "app",
-  -- Lean apparently needs help with this higher-order unification problem
-  apply definable.app_ctx' (λ d, (∧) (q.to_fun d ∧ p.to_fun d)) q.to_fun,
-
-  -- let's take care of the variable intro
+  defin_app,
   swap,
-  { exact q.definable },
-
-  -- now another app
-  apply definable.app_ctx' (λ d, (∧)) (λ d, (q.to_fun d ∧ p.to_fun d)),
-
-  -- a constant! look up the lemma somehow
+  { defin_var },
+  defin_app,
   { exact definable_const definable_and },
-
-  -- now the same game continues
-  apply definable.app_ctx' (λ d, (∧) (q.to_fun d)) p.to_fun,
-  { apply definable.app_ctx' (λ d, (∧)) q.to_fun,
+  defin_app,
+  { defin_app,
     { exact definable_const definable_and },
-    { exact q.definable } },
-  { exact p.definable }
+    defin_var },
+  { defin_var },
+end
 
+example : definable S (λ p q, (q ∧ p) ∧ q) :=
+begin [defin]
+  intro p,
+  intro q,
+  app,
+  swap,
+  { var },
+  app,
+  { exact definable_const definable_and },
+  app,
+  { app,
+    { exact definable_const definable_and },
+    var },
+  { var },
 end
 
 #exit
